---
aliases: 
tags:
title: Test
date created: Wednesday, August 3rd 2022, 11:27:17 am
date modified: Wednesday, August 3rd 2022, 11:27:20 am
---

# Test
$$
\begin{align*}
\ket{\rightarrow} &= 
\frac{1}{\sqrt{2}}(\ket{\uparrow}+\ket{\downarrow}) = \frac{1}{\sqrt{2}}\mqty[1 \\ 1]\\
\ket{\leftarrow} &= \frac{1}{\sqrt{2}}(\ket{\uparrow}-\ket{\downarrow}) = \frac{1}{\sqrt{2}}\mqty[1\\-1] \\
\ket{\odot} &= \frac{1}{\sqrt{2}}(\ket{\uparrow}+e^{i\eta}\ket{\downarrow} = \frac{1}{\sqrt{2}}\mqty[1 \\ e^{i\eta}] \\
\ket{\cross} &= \frac{1}{\sqrt{2}}(\ket{\uparrow}-e^{i\eta}\ket{\downarrow} = \frac{1}{\sqrt{2}} \mqty[1\\ -e^{i\eta}]
\end{align*}
$$
$$
\begin{align*}
\braket{\cross|\odot} &= \frac{1}{2}\mqty[1 & -e^{-i\eta}]\mqty[1 \\ e^{i\eta}] = 0 \\
|\braket{\rightarrow|\odot}|^2 &= \abs{\frac{1}{2}\mqty[1 & 1]\mqty[1 \\ e^{i\eta}]}^2 = \frac{1}{2} \\
\abs{1+e^{i\eta}}^2 &= 4 
\end{align*}
$$


